Lp2lc/Active/F.lean
@@ -1,1 +1,0 @@
-import «Lp2lc».Active.F.Def
