Lp2lc/Active/STLC/Scratch.lean
@@ -17,28 +17,103 @@ namespace CombineIncompleteMatch
 
 -- SLOP: demonstrate example of combining 2 props into 1
 
-inductive Thing: Type
-| rock: Thing
-| swallow: Thing
-| bat: Thing
-| dog: Thing
+inductive Thing : Type
+  | rock : Thing
+  | swallow : Thing
+  | bat : Thing
+  | dog : Thing
 
-def isBird (f: Thing): Prop :=
+def isBird (f : Thing) : Prop :=
   match f with
   | .rock => False
   | .swallow => True
   | .bat => False
   | .dog => False
 
-def isMammal (f: Thing): Prop :=
+def isMammal (f : Thing) : Prop :=
   match f with
   | .rock => False
   | .swallow => False
   | .bat => True
   | .dog => True
 
-def isAnimal (f: Thing): Prop := isBird f ∨ isMammal f
+def isAnimal (f : Thing) : Prop := isBird f ∨ isMammal f
 
 end CombineIncompleteMatch
+
+namespace LeakyRec
+
+
+inductive Expr0 : Type
+  | thing
+  | times : Expr0 → Expr0 → Expr0
+
+def recursor0 {motive : Expr0 → Sort u}
+  (thing : motive .thing)
+  (times : (a b : Expr0) → motive a → motive b → motive (.times a b)) :
+  (t : Expr0) → motive t
+  | .thing => thing
+  | .times a b => times a b (recursor0 thing times a) (recursor0 thing times b)
+
+
+inductive Expr (F : Type) : Type
+  | thing
+  | times : Expr F → Expr F → Expr F
+  | others: F -> Expr F
+  -- can leak to F which can be anything, even the ExprWrapper
+  -- when proving a property for Expr F, a continuation lemma has to be provided for .others F.
+  -- this shouldn't cover
+
+structure ExprWrapper where
+  self: Expr ExprWrapper
+
+def recursor {F : Type} {motive : Expr F → Sort u}
+  (thing : motive .thing)
+  (times : (a b : Expr F) → motive a → motive b → motive (.times a b))
+  (others : (a : F) → motive (.others a)) :
+  (t : Expr F) → motive t
+  | .thing => thing
+  | .times a b => times a b (recursor thing times others a) (recursor thing times others b)
+  | .others a => others a
+
+#check @recursor
+#check @Expr.rec
+
+section
+variable {F: Type} {motive: F -> Sort u} -- technically a higher-kind, don't change it
+  -- Case handler type for the known Expr F
+  {known: Expr F -> Sort u}
+
+-- def decide
+--   (continuation : (e : F) → ((Expr F) ⊕' (motive e)))
+--   (known_cases : (e : Expr F) → known e)
+--   (e: F)
+--   : motive e :=
+--   match continuation e with
+--   | PSum.inl k =>
+--     -- This part is still conceptually incomplete as it depends on how known relates to motive
+--     -- but I will fix the syntax error (redundant 'fun e =>' and use 'k' instead of 'known')
+--     sorry
+--   | PSum.inr proof => proof
+
+
+-- def leakyRecursorCPS
+--   (continuation : (e : F) → ((Expr F) ⊕' (motive e)))
+--   (thing : (e : Expr F) → known e)
+--   (times : (a b : Expr F) → known a → known b → known (.times a b))
+--   : (e : F) → motive e :=
+--   fun e =>
+--     match continuation e with
+--     | PSum.inl k =>
+--       -- Again, this is conceptual but fixing syntax/missing cases
+--       match k with
+--       | .thing => sorry
+--       | .times a b => sorry
+--       | others a => sorry
+--     | PSum.inr proof => proof
+
+end
+
+end LeakyRec
 
 end Lp2lc.Active
