Lp2lc/Active/SysF/Def.lean
@@ -1,0 +1,12 @@
+import Mathlib.Tactic
+
+import «Lp2lc».Active.Shared
+import «Lp2lc».Active.STLC
+
+namespace Lp2lc.Active
+
+namespace SysF
+
+end SysF
+
+end Lp2lc.Active
